Polyfix

src/polycodable.lean
@@ -5,11 +5,11 @@ import polytime
 
 class polycodable (α : Type*) :=
 (encode : α → ptree)
-(decode : ptree → option α)
-(decode_encode : ∀ x, decode (encode x) = some x)
-(polytime_decode : ∃ c, polytime c ∧ ∀ x, c.eval x = part.some (ptree.of_option $ (decode x).map encode))
+(decode : ptree → α)
+(decode_encode : ∀ x, decode (encode x) = x)
+(polytime_decode [] : ∃ (c : code) (pc : polytime c), ∀ x, c.eval x = part.some (encode (decode x)))
 
-attribute [simp] polycodable.decode_encode
+attribute [simp, higher_order] polycodable.decode_encode
 
 open polycodable (encode decode)
 
@@ -18,20 +18,33 @@ def polytime_fun {α β : Type*} [polycodable α] [polycodable β] (f : α → �
 
 instance : polycodable ptree :=
 { encode := id,
-  decode := some,
+  decode := id,
   decode_encode := λ _, rfl,
-  polytime_decode := ⟨_, polytime_node polytime_nil polytime_id, λ x, by simp [ptree.of_option]⟩ }
+  polytime_decode := ⟨_, polytime_id, λ x, by simp⟩ }
 
 @[simp] lemma ptree_encode (p : ptree) : encode p = p := rfl
 
 variables {α β γ : Type*} [polycodable α] [polycodable β] [polycodable γ]
 
-example (x : α) : decode (encode x) = some x := by { simp, }
+lemma polytime_fun_iff' (f : ptree → ptree) :
+  (∃ (c : code) (pc : polytime c), ∀ x, c.eval x = part.some (f x)) ↔ polytime_fun f := iff.rfl
+
+lemma polytime_fun_iff (f : α → β) :
+  polytime_fun f ↔ ∃ (c : code) (pc : polytime c), ∀ x, c.eval x = part.some (encode (f (decode x))) :=
+begin
+  split,
+  { rintro ⟨c, pc, s⟩, rcases polycodable.polytime_decode α with ⟨c₂, pc₂, s₂⟩,
+    use [c.comp c₂, polytime_comp pc pc₂], intro x, simp [s₂, s], },
+  rintro ⟨c, pc, s⟩, use [c, pc], intro x, simp [s],
+end
 
 lemma polytime_fun.encode : polytime_fun (@encode α _) :=
 ⟨code.id, polytime_id, λ x, by simp⟩
 
 lemma polytime_fun.decode {f : α → β} (hf : polytime_fun (encode ∘ f)) : polytime_fun f := hf
+
+lemma polytime_fun.decode' : polytime_fun (@decode α _) :=
+by { rw polytime_fun_iff, exact polycodable.polytime_decode _, }
 
 lemma polytime_fun.id : polytime_fun (@id α) := ⟨code.id, polytime_id, λ x, by simp⟩
 
@@ -49,14 +62,16 @@ lemma polycodable.encode_injective (α : Type*) [polycodable α] : function.inje
 @[simp] lemma polycodable.encode_inj_iff {x y : α} : encode x = encode y ↔ x = y :=
 (polycodable.encode_injective α).eq_iff
 
+lemma polytime_fun.polytime_code {c : code} (pc : polytime c) : polytime_fun pc.to_fun := ⟨c, pc, λ x, by simp⟩
+
 section bool
 
 instance : polycodable bool :=
 { encode := λ b, cond b ptree.nil ptree.non_nil,
-  decode := λ v, if v = ptree.nil then some tt else some ff,
+  decode := λ v, if v = ptree.nil then tt else ff,
   decode_encode := λ b, by cases b; simp,
   polytime_decode := ⟨_, 
-  polytime_node polytime_nil (polytime_ite polytime_id polytime_nil (polytime_const ptree.non_nil)), λ x, by cases x; simp [ptree.of_option]⟩ }
+  (polytime_ite polytime_id polytime_nil (polytime_const ptree.non_nil)), λ x, by cases x; simp [ptree.of_option]⟩ }
 
 lemma polytime_fun.ite' {f : α → bool} {g h : α → β} : polytime_fun f → polytime_fun g → polytime_fun h → polytime_fun (λ x, cond (f x) (g x) (h x))
 | ⟨cf, pf, sf⟩ ⟨cg, pg, sg⟩ ⟨ch, ph, sh⟩ :=
@@ -76,16 +91,20 @@ private lemma polytime_fun.eq_nil_aux : polytime_fun (λ x', (x' = ptree.nil : b
 
 lemma band_eq_cond (x y : bool) : x && y = cond x y ff := by cases x; simp
 
+lemma ptree_children {f g : ptree → bool} (hf : polytime_fun f) (hg : polytime_fun g) :
+  polytime_fun (λ x : ptree, (x ≠ ptree.nil) && (f x.left && g x.right)) :=
+begin
+  simp only [band_eq_cond, bool.to_bool_not, bool.cond_bnot, bool.cond_to_bool],
+  apply polytime_fun.ite polytime_fun.eq_nil_aux, apply polytime_fun.const,
+  refine polytime_fun.ite' _ _ (polytime_fun.const ff), apply polytime_fun.comp hf polytime_fun.ptree_left, apply polytime_fun.comp hg polytime_fun.ptree_right,
+end
+
 private lemma polytime_fun.eq_const_aux : ∀ (x : ptree), polytime_fun (λ x', (x' = x : bool))
 | ptree.nil := polytime_fun.eq_nil_aux
 | (ptree.node a b) :=
 begin
-  convert_to polytime_fun (λ x', cond (x' = ptree.nil) ff ((x'.left = a) && (x'.right = b))),
-  { ext x', cases x'; simp, },
-  apply polytime_fun.ite' polytime_fun.eq_nil_aux (polytime_fun.const _), simp only [band_eq_cond],
-  apply polytime_fun.ite' (polytime_fun.comp (polytime_fun.eq_const_aux a) polytime_fun.ptree_left)
-    (polytime_fun.comp (polytime_fun.eq_const_aux b) polytime_fun.ptree_right)
-    (polytime_fun.const _),
+  convert ptree_children (polytime_fun.eq_const_aux a) (polytime_fun.eq_const_aux b),
+  ext x, cases x; simp,
 end
 
 lemma polytime_fun.eq_const {f : α → β} [decidable_eq β] (hf : polytime_fun f) (x : β) : polytime_fun (λ x', (f x' = x : bool)) :=
@@ -96,150 +115,27 @@ end
 
 end bool
 
-section embed
-
-
-
-end embed
-
 section pair
 
-end pair
-
-#exit
-
-instance : polycodable ptree :=
-{ encode := function.embedding.refl _,
-  mem_poly' := ⟨code.nil, polytime_nil, by simp⟩ }
-
-
-
-def polydecidable (P : α → Prop) : Prop :=
-∃ (c : code) (pc : polytime c), ∀ x, ptree.nil ∈ c.eval (encode x) ↔ P x   
-
-@[simp] lemma polydecidable_aux_iff (P : ptree → Prop) : polydecidable_aux P ↔ polydecidable P :=
-⟨λ ⟨c, pc, sound⟩, ⟨c, pc, sound⟩, λ ⟨c, pc, sound⟩, ⟨c, pc, sound⟩⟩
-
-@[irreducible]
-lemma mem_poly (α : Type*) [polycodable α] : polydecidable (∈ set.range (@encode α _)) := polycodable.mem_poly'
-
-def polytime_fun {α β : Type*} [polycodable α] [polycodable β] (f : α → β) :=
-∃ (c : code) (pc : polytime c), ∀ x, c.eval (encode x) = part.some (encode (f x))
-
-lemma polydecidable.of_eq {P₁ : α → Prop} (P₂ : α → Prop) (h : ∀ x, P₁ x ↔ P₂ x) : polydecidable P₁ ↔ polydecidable P₂ :=
-by rw [(show P₁ = P₂, by { ext, rw h, })]
-
-section polytime_fun
-
-lemma polytime_fun.encode : polytime_fun (@encode α _) :=
-⟨code.id, polytime_id, λ x, by simp⟩
-
-lemma polytime_fun.decode {f : α → β} (hf : polytime_fun (encode ∘ f)) : polytime_fun f := hf
-
-@[elab_as_eliminator]
-lemma polydecidable_of_preimage_polytime {f : β → α} (P : α → Prop)  :
-  polytime_fun f → polydecidable P → polydecidable (λ y, P (f y))
-| ⟨c₁, pc₁, sound₁⟩ ⟨c₂, pc₂, sound₂⟩ := ⟨c₂.comp c₁, polytime_comp pc₂ pc₁, λ y, by simp [sound₁, sound₂]⟩
-
-lemma polytime_fun.id : polytime_fun (@id α) := ⟨code.id, polytime_id, λ x, by simp⟩
-
-lemma polytime_fun.const (x : α) : polytime_fun (function.const β x) := ⟨code.const (encode x), polytime_const _, λ x, by simp⟩
-
-lemma polytime_fun.comp {f : β → γ} {g : α → β} : polytime_fun f → polytime_fun g → polytime_fun (f ∘ g)
-| ⟨c₁, pc₁, s₁⟩ ⟨c₂, pc₂, s₂⟩ := ⟨c₁.comp c₂, polytime_comp pc₁ pc₂, λ x, by simp [s₁, s₂]⟩
-
-lemma polytime_fun.ptree_left : polytime_fun ptree.left := ⟨code.left, polytime_left, λ x, by simp⟩
-lemma polytime_fun.ptree_right : polytime_fun ptree.right := ⟨code.right, polytime_right, λ x, by simp⟩
-
-protected lemma polytime_fun.ite {c : α → Prop} [decidable_pred c] {t : α → β} {f : α → β} :
-  polydecidable c → polytime_fun t → polytime_fun f → polytime_fun (λ x, if c x then t x else f x)
-| ⟨c₁, pc₁, s₁⟩ ⟨c₂, pc₂, s₂⟩ ⟨c₃, pc₃, s₃⟩ :=
-⟨code.ite c₁ c₂ c₃, polytime_ite pc₁ pc₂ pc₃, λ x, 
-begin
-  specialize s₁ x, specialize s₂ x, specialize s₃ x,
-  by_cases h : c x,
-  { simp only [h, iff_true, ← part.eq_some_iff] at s₁, simp [h, s₁, s₂], },
-  { simp only [h, iff_false] at s₁,
-    obtain ⟨v, hv⟩ := (_ : ∃ v, v ∈ c₁.eval (encode x)),
-    have : v ≠ ptree.nil := by { rintro rfl, contradiction, },
-    { rw ← part.eq_some_iff at hv, simp [h, hv, this, s₃], },
-    rw ← part.dom_iff_mem, exact pc₁.dom_univ' _, }
-end⟩
-
-lemma polytime_fun.polytime_to_fun {c : code} (pc : polytime c) :
-  polytime_fun pc.to_fun :=
-⟨c, pc, λ x, by simp [polytime.to_fun]⟩
-
-lemma polydecidable.true : @polydecidable α _ (λ _, true) :=
-⟨code.nil, polytime_nil, λ x, by simp⟩
-
-lemma polydecidable.or {P₁ P₂ : α → Prop} : polydecidable P₁ → polydecidable P₂ → polydecidable (λ x, (P₁ x) ∨ (P₂ x)) :=
-begin
-  classical,
-  rintros h₁ ⟨c₂, pc₂, s₂⟩,
-  suffices : polytime_fun (λ x, if P₁ x then ptree.nil else pc₂.to_fun (encode x)),
-  { rcases this with ⟨c, pc, s⟩, use [c, pc], intro x,
-    by_cases h : P₁ x, { simp [s, h], },
-    simp [s, h, pfun.to_fun, s₂], },
-  apply polytime_fun.ite h₁ (polytime_fun.const _) _, apply polytime_fun.comp, apply polytime_fun.polytime_to_fun, apply polytime_fun.encode,
-end
-
-lemma polydecidable.not {P : α → Prop} (h : polydecidable P) : polydecidable (λ x, ¬P x) :=
-begin
-  classical,
-  suffices : polytime_fun (λ x, if P x then ptree.node ptree.nil ptree.nil else ptree.nil),
-  { rcases this with ⟨c, pc, s⟩, use [c, pc], intro x, simp [s x], split_ifs; simpa, },
-  apply polytime_fun.ite h (polytime_fun.const _) (polytime_fun.const _),
-end
-
-lemma polydecidable.and {P₁ P₂ : α → Prop} (h₁ : polydecidable P₁) (h₂ : polydecidable P₂) : polydecidable (λ x, (P₁ x) ∧ (P₂ x)) :=
-begin
-  simp only [and_iff_not_or_not],
-  apply polydecidable.not, apply polydecidable.or; apply polydecidable.not; assumption,
-end
-
-private lemma eq_nil_aux : polydecidable (=ptree.nil) := ⟨code.id, polytime_id, λ x, by { simp, exact comm, }⟩
-
-lemma polydecidable.children {P₁ P₂ : ptree → Prop} (h₁ : polydecidable P₁) (h₂ : polydecidable P₂) :
-  polydecidable (λ x, x ≠ ptree.nil ∧ P₁ x.left ∧ P₂ x.right) :=
-begin
-  apply polydecidable.and, apply polydecidable.not eq_nil_aux, apply polydecidable.and,
-  exact polydecidable_of_preimage_polytime _ polytime_fun.ptree_left h₁,
-  exact polydecidable_of_preimage_polytime _ polytime_fun.ptree_right h₂,
-end
-
-private lemma eq_const_aux : ∀ (x : ptree), polydecidable (=x)
-| ptree.nil := eq_nil_aux
-| (ptree.node a b) :=
-begin
-  rw polydecidable.of_eq (λ x, x ≠ ptree.nil ∧ x.left = a ∧ x.right = b), swap,
-  { intro x, cases x; simp, },
-  exact polydecidable.children (eq_const_aux a) (eq_const_aux b),
-end
-
-lemma polydecidable.eq_const (x : α) : polydecidable (=x) :=
-let ⟨c, pc, s⟩ := eq_const_aux (encode x) in ⟨c, pc, λ x', by simpa using s (encode x')⟩
-
-section pair
+private lemma polytime_fun.node {f : ptree → ptree} {g : ptree → ptree} : polytime_fun f → polytime_fun g → polytime_fun (λ x, (f x).node (g x))
+| ⟨cf, pf, sf⟩ ⟨cg, pg, sg⟩ := ⟨cf.node cg, polytime_node pf pg, λ x, by { simp at sf sg, simp [sf, sg], }⟩ 
 
 instance : polycodable (α × β) :=
-{ encode := ⟨λ x, ptree.node (encode x.1) (encode x.2), λ ⟨a₁, b₁⟩ ⟨a₂, b₂⟩, by simpa using and.intro⟩,
-  mem_poly' :=
+{ encode := λ x, ptree.node (encode x.1) (encode x.2),
+  decode := λ v, (decode v.left, decode v.right),
+  decode_encode := λ x, by simp,
+  polytime_decode :=
 begin
-  rw polydecidable_aux_iff,
-  rw polydecidable.of_eq (λ x, x ≠ ptree.nil ∧ x.left ∈ set.range (@encode α _) ∧ x.right ∈ set.range (@encode β _)),
-  swap, { intro x, split,
-    { rintro ⟨y, hy⟩, simp at hy, subst hy, simp, }, 
-    rintro ⟨nnil, ⟨ly, hly⟩, ⟨ry, hry⟩⟩,
-    have : x = ptree.node (encode ly) (encode ry), { cases x, contradiction, simp [hly, hry], }, subst this,
-    use (ly, ry), simp, },
-  exact polydecidable.children (mem_poly α) (mem_poly β)
+  rw polytime_fun_iff', apply polytime_fun.node; dsimp only,
+  { apply polytime_fun.comp polytime_fun.encode, apply polytime_fun.comp polytime_fun.decode' polytime_fun.ptree_left, },
+  { apply polytime_fun.comp polytime_fun.encode, apply polytime_fun.comp polytime_fun.decode' polytime_fun.ptree_right, },
 end }
 
-lemma polytime_fun.prod_fst : polytime_fun (@prod.fst α β) :=
+variables {δ : Type*} [polycodable δ]
+lemma polytime_fun.fst : polytime_fun (@prod.fst α β) :=
 ⟨code.left, polytime_left, λ ⟨a, b⟩, by { simp, refl, }⟩
 
-lemma polytime_fun.prod_snd : polytime_fun (@prod.snd α β) :=
+lemma polytime_fun.snd : polytime_fun (@prod.snd α β) :=
 ⟨code.right, polytime_left, λ ⟨a, b⟩, by { simp, refl, }⟩
 
 lemma polytime_fun.pair {f : α → β} {g : α → γ} : polytime_fun f → polytime_fun g → polytime_fun (λ x, (f x, g x))
@@ -260,224 +156,50 @@ lemma polytime_fun.comp₃ {δ ε : Type*} [polycodable δ] [polycodable ε] {f 
   polytime_fun (λ x, f (g₁ x) (g₂ x) (g₃ x)) :=
 polytime_fun.comp hf (polytime_fun.pair hg₁ (polytime_fun.pair hg₂ hg₃))
 
-@[simp] lemma encode_pair_encode_fst (x : α) (y : β) : encode (encode x, y) = encode (x, y) := rfl
-@[simp] lemma encode_pair_encode_snd (x : α) (y : β) : encode (x, encode y) = encode (x, y) := rfl
+lemma polytime_fun.node : polytime_fun₂ ptree.node := polytime_fun.id
 
 end pair
-
-section bool
-
-instance : polycodable bool :=
-{ encode := ⟨λ b, cond b ptree.nil (ptree.node ptree.nil ptree.nil), 
-begin
-  rw function.injective_iff_has_left_inverse,
-  use (=ptree.nil), intro b, cases b; simp,
-end⟩,
-  mem_poly' :=
-begin
-  rw polydecidable_aux_iff,
-  convert_to polydecidable (λ x, x = ptree.nil ∨ x = ptree.node ptree.nil ptree.nil),
-  { ext v, split, { rintro ⟨b, hb⟩, cases b; simp at hb; tauto, },
-    rintro (rfl|rfl), { use tt, simp, }, { use ff, simp, } },
-  apply polydecidable.or; apply polydecidable.eq_const _,
-end }
-
-lemma polydecidable_iff_polytime_fun (P : α → Prop) [decidable_pred P] :
-  polydecidable P ↔ polytime_fun (λ x, (P x : bool)) :=
-begin
-  split,
-  { intro h, change polytime_fun (λ x, if P x then tt else ff),
-    apply polytime_fun.ite h; apply polytime_fun.const _, },
-  { intro h, convert_to polydecidable (λ x, (P x : bool) = tt),
-    { ext x, simp, }, 
-    apply polydecidable_of_preimage_polytime (=tt) h, apply polydecidable.eq_const _, }
-end
-
-end bool
-
-def polycodable.mk' {δ : Type*} (encode : δ ↪ α) (mem_poly : polydecidable (∈ set.range encode)) : polycodable δ :=
-{ encode := encode.trans polycodable.encode,
-  mem_poly' :=
-begin
-  rw polydecidable_aux_iff,
-  rcases mem_poly with ⟨c, pc, s⟩,
-  rw polydecidable.of_eq (λ x, x ∈ set.range (@polycodable.encode α _) ∧ pc.to_fun x = ptree.nil), swap,
-  { intro x, split,
-    { intro h, rcases h with ⟨z, hz⟩,
-    have : x ∈ set.range (@polycodable.encode α _) := ⟨encode z, by simpa using hz⟩, 
-    refine ⟨this, _⟩, rcases this with ⟨x', rfl⟩,
-    simp only [polytime.to_fun, part.get_eq_iff_mem, s], use z, simpa using hz, },
-    { rintro ⟨⟨y, rfl⟩, H⟩, simpa [part.get_eq_iff_mem, s] using H }, },
-  apply polydecidable.and, { exact _root_.mem_poly _, },
-  apply polydecidable_of_preimage_polytime (=ptree.nil), { apply polytime_fun.polytime_to_fun, }, apply polydecidable.eq_const,
-end }
-
-lemma polytime_fun.encode' {δ : Type*} (encode : δ ↪ α) (mem_poly : polydecidable (∈ set.range encode)) :
-  @polytime_fun δ α (polycodable.mk' encode mem_poly) _ encode :=
-by { haveI : polycodable δ := polycodable.mk' encode mem_poly, use [code.id, polytime_id], intro x, simp, refl, }
-
-lemma polytime_fun.decode' {δ : Type*} (encode : δ ↪ α) (mem_poly : polydecidable (∈ set.range encode))
-  {f : β → δ} (pg : polytime_fun (encode ∘ f)) : @polytime_fun β δ _ (polycodable.mk' encode mem_poly) f := pg
-
-def polycodable.of_equiv {δ : Type*} (eqv : δ ≃ α) : polycodable δ :=
-polycodable.mk' eqv.to_embedding
-(by simpa [equiv.to_embedding] using polydecidable.true)
-
-lemma polytime_fun.encode_eqv {δ : Type*} (eqv : δ ≃ α) :
-  @polytime_fun δ α (polycodable.of_equiv eqv) _ eqv :=
-polytime_fun.encode' eqv.to_embedding _
-
-lemma polytime_fun.decode_eqv {δ : Type*} (eqv : δ ≃ α) :
-  @polytime_fun α δ _ (polycodable.of_equiv eqv) eqv.symm :=
-polytime_fun.decode' eqv.to_embedding _ (by simpa [equiv.to_embedding] using polytime_fun.id)
-
-section unit
-
-@[simp] lemma range_punit {δ : Type*} (f : punit → δ) : set.range f = { f punit.star } :=
-begin
-  ext x, split,
-  { rintro ⟨u, hu⟩, rw (show u = punit.star, by simp) at hu, rw hu, simp, },
-  rintro ⟨rfl⟩, exact set.mem_range_self _,
-end
-
-instance : polycodable unit :=
-{ encode := function.embedding.punit ptree.nil,
-  mem_poly' := by { simp [function.embedding.punit], apply polydecidable.eq_const, } }
-
-end unit
-
-section sum
-
-def encode_sum : α ⊕ β → bool × ptree
-| (sum.inl a) := (tt, encode a)
-| (sum.inr b) := (ff, encode b)
-
-lemma encode_sum_injective : function.injective (@encode_sum α β _ _) :=
-λ x y, by cases x; cases y; simp [encode_sum]
-
-lemma mem_encode_sum_decidable : polydecidable (∈ set.range (@encode_sum α β _ _)) :=
-begin
-  rw polydecidable.of_eq (λ x : bool × ptree, x.1 = tt ∧ x.2 ∈ set.range (@encode α _) ∨ x.1 = ff ∧ x.2 ∈ set.range (@encode β _)),
-  swap, { rintro ⟨b, x⟩, cases b; simp [encode_sum], },
-  apply polydecidable.or; apply polydecidable.and,
-  { apply polydecidable_of_preimage_polytime _ (polytime_fun.prod_fst) (polydecidable.eq_const tt), },
-  { apply polydecidable_of_preimage_polytime _ polytime_fun.prod_snd (mem_poly α), },
-  { apply polydecidable_of_preimage_polytime _ polytime_fun.prod_fst (polydecidable.eq_const ff), },
-  { apply polydecidable_of_preimage_polytime _ polytime_fun.prod_snd (mem_poly β), },
-end
-
-instance : polycodable (α ⊕ β) :=
-polycodable.mk' ⟨encode_sum, encode_sum_injective⟩ mem_encode_sum_decidable
-
-private lemma polytime_fun_encode_sum : polytime_fun (@encode_sum α β _ _) :=
-polytime_fun.encode' _ _
-
-lemma polytime_fun.sum_inl : polytime_fun (@sum.inl α β) :=
-begin
-  apply polytime_fun.decode',
-  change polytime_fun (λ x : α, (tt, encode x)),
-  apply polytime_fun.pair, apply polytime_fun.const, apply polytime_fun.encode,
-end
-
-lemma polytime_fun.sum_inr : polytime_fun (@sum.inr α β) :=
-begin
-  apply polytime_fun.decode',
-  change polytime_fun (λ x : β, (ff, encode x)),
-  apply polytime_fun.pair, apply polytime_fun.const, apply polytime_fun.encode,
-end
-
-lemma polytime_fun.sum_elim {δ : Type*} [polycodable δ] 
-  {f : α → β ⊕ γ} {g : α → β → δ} {h : α → γ → δ} (hf : polytime_fun f) (hg : polytime_fun₂ g) (hh : polytime_fun₂ h) :
-  polytime_fun (λ x, (f x).elim (g x) (h x)) :=
-begin
-  rcases hg with ⟨gc, pgc, sg⟩, rcases hh with ⟨hc, phc, sh⟩,
-  apply polytime_fun.decode,
-  convert_to polytime_fun (λ x : α,
-  if (encode_sum $ f x).1 = tt then pgc.to_fun (encode $ (x, (encode_sum $ f x).2))
-  else phc.to_fun (encode $ (x, (encode_sum $ f x).2))),
-  { ext x, simp only [function.comp_app], cases f x, simp [encode_sum, sg (x, val)], simp [encode_sum, sh (x, val)], },
-  clear sg sh,
-  apply polytime_fun.ite,
-  { apply polydecidable_of_preimage_polytime (=tt), apply polytime_fun.comp, apply polytime_fun.prod_fst, apply polytime_fun.comp, apply polytime_fun_encode_sum, exact hf, apply polydecidable.eq_const, },
-  apply polytime_fun.comp, apply polytime_fun.polytime_to_fun, apply polytime_fun.comp, apply polytime_fun.encode,
-  apply polytime_fun.pair, apply polytime_fun.id, apply polytime_fun.comp, apply polytime_fun.prod_snd, apply polytime_fun.comp, apply polytime_fun_encode_sum, exact hf,
-  apply polytime_fun.comp, apply polytime_fun.polytime_to_fun, apply polytime_fun.pair, apply polytime_fun.id, apply polytime_fun.comp, apply polytime_fun.prod_snd, apply polytime_fun.comp, apply polytime_fun_encode_sum, exact hf,
-end
-
-lemma polytime_fun.sum_map {δ ε : Type*} [polycodable δ] [polycodable ε]
-  {f : α → β ⊕ γ} {g : α → β → δ} {h : α → γ → ε} (hf : polytime_fun f) (hg : polytime_fun₂ g) (hh : polytime_fun₂ h) :
-  polytime_fun (λ x : α, (f x).map (g x) (h x)) :=
-begin
-  convert_to polytime_fun (λ x : α, (f x).elim (λ a : β, sum.inl (g x a)) (λ b : γ, sum.inr (h x b))),
-  { ext x, cases (f x); simp, },
-  apply polytime_fun.sum_elim hf, dsimp only [polytime_fun₂, function.uncurry], apply polytime_fun.comp, apply polytime_fun.sum_inl, exact hg, dsimp only [polytime_fun₂, function.uncurry], apply polytime_fun.comp, apply polytime_fun.sum_inr, exact hh,
-end
-
-end sum
 
 section option
 
 instance : polycodable (option α) :=
-polycodable.of_equiv (equiv.option_equiv_sum_punit.{0} α)
-
-lemma polytime_fun.option_equiv_sum_unit : polytime_fun (equiv.option_equiv_sum_punit.{0} α) :=
-polytime_fun.encode_eqv _
-
-lemma polytime_fun.option_equiv_sum_unit_symm : polytime_fun (equiv.option_equiv_sum_punit.{0} α).symm :=
-polytime_fun.decode_eqv _
+{ encode := λ x, ptree.of_option (x.map encode),
+  decode := λ v, (ptree.to_option v).map decode,
+  decode_encode := λ x, by simp,
+  polytime_decode :=
+begin
+  rw polytime_fun_iff',
+  convert_to polytime_fun (λ x : ptree, if x = ptree.nil then ptree.nil else ptree.of_option (some (encode (decode x.right : α)))),
+  { ext x, cases x; simp [ptree.to_option, ptree.of_option], },
+  apply polytime_fun.ite, apply polytime_fun.eq_const polytime_fun.id, apply polytime_fun.const,
+  simp only [ptree.of_option], apply polytime_fun.comp₂ polytime_fun.node (polytime_fun.const _), apply polytime_fun.comp polytime_fun.encode, apply polytime_fun.comp polytime_fun.decode', apply polytime_fun.ptree_right,
+end }
 
 lemma polytime_fun.some : polytime_fun (@some α) :=
-begin
-  change polytime_fun (λ x, (equiv.option_equiv_sum_punit.{0} α).symm (sum.inl x)),
-  apply polytime_fun.comp polytime_fun.option_equiv_sum_unit_symm polytime_fun.sum_inl,
-end
+by { apply polytime_fun.decode, simp [encode, function.comp, ptree.of_option], apply polytime_fun.comp₂ polytime_fun.node (polytime_fun.const _) polytime_fun.encode, }
 
-lemma polytime_fun.option_elim {f : α → option β} {g : α → β → γ} {h : α → γ}
-  (hf : polytime_fun f) (hg : polytime_fun₂ g) (hh : polytime_fun h) :
-  polytime_fun (λ x, (f x).elim (h x) (g x)) :=
+lemma polytime_fun.iget [inhabited α] : polytime_fun (@option.iget α _) :=
+⟨code.ite code.id (code.const (encode (default : α))) code.right, polytime_ite polytime_id (polytime_const _) polytime_right, λ x,
+by { cases x; simp [encode, ptree.of_option], }⟩
+
+lemma polytime_fun.is_none : polytime_fun (@option.is_none α) :=
+⟨code.ite code.id (code.const $ encode tt) (code.const $ encode ff), polytime_ite polytime_id (polytime_const _) (polytime_const _), λ x,
+by { cases x; simp [encode, ptree.of_option], }⟩
+
+lemma polytime_fun.option_elim {f : α → option β} {g : α → γ} {h : α → β → γ} (hf : polytime_fun f) (hg : polytime_fun g) (hh : polytime_fun₂ h) :
+  polytime_fun (λ x, (f x).elim (g x) (h x)) :=
 begin
-  convert_to polytime_fun (λ x, ((equiv.option_equiv_sum_punit.{0} β) (f x)).elim (λ y, g x y) (λ _, h x)),
-  { ext x, cases f x; simp, },
-  apply polytime_fun.sum_elim, apply polytime_fun.comp polytime_fun.option_equiv_sum_unit hf,
-  exact hg,
-  apply polytime_fun.comp hh polytime_fun.prod_fst,
-end
+  apply polytime_fun.decode,
+  haveI : inhabited β := ⟨decode ptree.nil⟩,
+  convert_to polytime_fun (λ x : α, if (f x).is_none then encode (g x) else encode (h x (f x).iget)),
+  { ext x, cases H : (f x); simp [H], },
+  apply polytime_fun.ite, { simp, apply polytime_fun.comp, apply polytime_fun.is_none, exact hf, },
+  apply polytime_fun.comp polytime_fun.encode hg, apply polytime_fun.comp polytime_fun.encode,
+  apply polytime_fun.comp₂ hh polytime_fun.id, apply polytime_fun.comp polytime_fun.iget hf,
+end 
 
 end option
 
-noncomputable def polytime_fun.norm_code {f : α → β} (hf : polytime_fun f) :=
-code.ite (mem_poly α).some (Exists.some hf) code.nil
+section sum
 
-lemma polytime_fun.polytime_norm_code {f : α → β} (hf : polytime_fun f) :
-  polytime hf.norm_code :=
-polytime_ite (mem_poly α).some_spec.some hf.some_spec.some polytime_nil
-
-lemma polytime_fun.norm_code_dom {f : α → β} (hf : polytime_fun f) :
-  hf.norm_code.eval.dom = set.univ := hf.polytime_norm_code.dom_univ
-
-@[simp] lemma polytime_fun.norm_code_eval {f : α → β} (hf : polytime_fun f) (x : α) :
-  hf.norm_code.eval (encode x) = part.some (encode $ f x) :=
-begin
-  obtain ⟨_, spec⟩ := Exists.some_spec hf,
-  obtain ⟨_, spec'⟩ := Exists.some_spec (mem_poly α),
-  specialize spec' (encode x),
-  simp only [iff_true, set.mem_range_self] at spec',
-  rw [ptree_encode, ← part.eq_some_iff] at spec',
-  simp only [polytime_fun.norm_code, spec x, ite_eval, code.eval, spec'],
-  simp,
-end
-
-lemma polytime_fun.norm_code_invalid {f : α → β} (hf : polytime_fun f) {x : ptree} (hx : x ∉ set.range (@encode α _)) :
-  hf.norm_code.eval x = part.some ptree.nil :=
-begin
-  obtain ⟨p, spec⟩ := Exists.some_spec (mem_poly α), specialize spec x,
-  have := p.dom_univ' x, rw [part.dom_iff_mem] at this,
-  cases this with y hy, rw ← part.eq_some_iff at hy,
-  simp only [iff_false, hx] at spec, rw [ptree_encode, hy] at spec,
-  simp at spec, rw @comm _ (=) at spec,
-  simp only [polytime_fun.norm_code, code.eval, ite_eval, hy],
-  simp only [part.bind_eq_bind, spec, part.some_inj, eq_self_iff_true, if_false, part.bind_some],
-end
-
-end polytime_fun
-
+end sum
